trying with new definitions

developmentCS/Hoare_initVAddrTable.v
@@ -158,6 +158,39 @@ intros.
 contradiction.
 Qed.
 
+Definition THoareFunTriple_Eval
+      (P: W -> Prop) (Q: Value -> W -> Prop) 
+      (fenv: funEnv) (env: valEnv)
+      (qf: QFun) : Prop :=
+  forall (ftenv: funTC)
+         (k1: FEnvTyping fenv ftenv)
+         (ft: FTyp)
+         (k2: QFunTyping ftenv fenv qf ft)
+         (s s': W) (f: Fun),
+  QFClosure fenv (Conf QFun s qf) (Conf QFun s' (QF f)) ->
+  match f with
+    | FC fenv' tenv' e0 e1 x n => 
+    EnvTyping env tenv' ->  
+    match n with
+      | 0 =>       
+        THoareTriple_Eval P Q fenv' env e0
+      | S n' =>       
+        THoareTriple_Eval P Q ((x,FC fenv' tenv' e0 e1 x n')::fenv')
+                           env e1
+    end
+  end.
+
+
+Lemma Apply_VHTT2 (P0: W -> Prop) (P1: list Value -> W -> Prop)
+                 (P2: Value -> W -> Prop) 
+   (fenv: funEnv) (env: valEnv) (qf: QFun) (es: list Exp) :
+  THoarePrmsTriple_Eval P0 P1 fenv env (PS es) ->
+  (forall env, THoareFunTriple_Eval (P1 (map snd env)) P2 fenv env qf) -> 
+  THoareTriple_Eval P0 P2 fenv env (Apply qf (PS es)).
+Proof.
+Admitted.
+
+
 
 (******* Hoare Triple *)
 
@@ -169,18 +202,7 @@ fenv >> env >> initVAddrTable table curidx
 Proof.
 unfold initVAddrTable.
 unfold initVAddrTableAux.
-assert(Hsize : tableSize + curidx >= tableSize) by omega.
-revert Hsize.
-revert table curidx.
-generalize tableSize at 1 3. 
-induction n.  simpl. 
-(** begin case n=0 *)
-intros.
-destruct curidx.
-simpl in *.
-omega.
-intros table curidx H.
-eapply Apply_VHTT1.
+eapply Apply_VHTT2.
 (** begin PS [Val (cst index curidx)] *)
 instantiate (1:= fun vs s => (forall idx : index,
    idx < curidx -> readVirtual table idx (memory s) = Some defaultVAddr) 
@@ -188,14 +210,30 @@ instantiate (1:= fun vs s => (forall idx : index,
 unfold THoarePrmsTriple_Eval.
 intros.
 inversion X;subst.
-destruct vs; inversion H6.
-destruct vs ; inversion H3 ; subst.
+destruct vs; inversion H5.
+destruct vs ; inversion H2 ; subst.
 intuition.
 inversion X0;subst.
 inversion X2.
 inversion X2.
 (** end *)
-intuition;simpl.
+intros vs ; simpl.
+unfold THoareFunTriple_Eval;intros.
+inversion X;subst.
+Focus 2. inversion X0.
+revert vs.
+assert(H : tableSize + curidx >= tableSize) by omega.
+revert H.
+revert curidx.
+generalize tableSize at 1 3. 
+induction n.  simpl. 
+(** begin case n=0 *)
+intros.
+destruct curidx.
+simpl in *.
+omega.
+(** end *)
+intros;simpl.
 destruct vs.
 unfold THoareTriple_Eval;intros.
 intuition; inversion H2.
@@ -203,13 +241,17 @@ destruct vs.
 Focus 2.
 unfold THoareTriple_Eval;intros.
 intuition; inversion H2.
+destruct p.
+simpl in *.
+inversion X0;subst.
+clear X1 H1.
 eapply BindN_VHTT1.
 (** Begin write Virtual *)
 unfold THoareTriple_Eval.
 intros.
-clear k3 k2 k1 t tenv ftenv.
+clear X0 X IHn k4 k3 k2 k1 k0 t ft ftenv ftenv0 tenv env.
+rename X1 into X.
 intuition.
-subst.
 inversion H2;subst.
 inversion X;subst.
 inversion X1;subst.
@@ -273,6 +315,7 @@ inversion X5.
 eapply IfTheElse_VHTT1.
 (** begin LtLtb *)
 unfold THoareTriple_Eval.
+clear X IHn k2 k1 ft env ftenv X0.
 intros.
 clear k3 k2 k1 t tenv ftenv.
 intuition.
@@ -302,9 +345,10 @@ intuition.
 inversion X5.
 inversion X5.
 (** end *)
-unfold mkVEnv;simpl.
+simpl.
 eapply BindS_VHTT1.
 eapply BindS_VHTT1.
+clear IHn X k2 k1 ft env ftenv X0.
 (** begin SuccD *)
 eapply weakenEval.
 instantiate (2:= fun s => (fun s' => (forall idx : index,
@@ -330,6 +374,7 @@ omega.
 (** end *) 
 (** begin ExtractIndex *)
 intros;simpl.
+clear IHn X k2 k1 ft env ftenv X0.
 instantiate (1:= fun v' s => (forall idx : index,
    idx < curidx -> readVirtual table idx (memory s) = Some defaultVAddr) /\
    readVirtual table curidx (memory s) = Some defaultVAddr /\
@@ -369,71 +414,82 @@ inversion X5.
 inversion X5.
 (** end *)
 intros; simpl.
+clear X.
 (** ending calls *)
 unfold THoareTriple_Eval.
 intros.
-destruct curidx.
-specialize (IHn table (CIndex(i+1))).
-eapply IHn.
-clear IHn X k3 k2 k1 t tenv ftenv.
+admit.
+(*destruct curidx.
 simpl in *.
-unfold CIndex.
-destruct (lt_dec (i+1) tableSize).
-simpl.
-omega.
-omega.
+specialize (IHn (CIndex(i+1))).
 simpl in *.
-instantiate (1:=ftenv).
+unfold CIndex in *.
+case_eq (lt_dec (i + 1) tableSize);intros.
+rewrite H1 in *.
+simpl in *.
+assert (Z : n+(i+1) = S(n+i)) by omega.
+rewrite Z in *.
+eapply IHn in H as H5.
+clear IHn.
+destruct n eqn:B.
+omega.
+eapply H5.
+admit.
+eauto.
 admit.
 admit.
 admit.
-admit.
-(*
-clear IHn k3 k2 k1 t tenv ftenv.
-inversion X;subst.
-inversion X0;subst.
-inversion X2;subst.
-inversion X3;subst.
-inversion H1;subst.
-clear X3 H1.
+instantiate (1:=v0).
 inversion X1;subst.
-inversion X3;subst.
-inversion H12;subst.
-destruct vs; inversion H1.
-inversion H12;subst.
-destruct vs; inversion H1.
+inversion X2;subst.
+inversion X4;subst.
 inversion X5;subst.
-inversion X6;subst.
+inversion H1;subst.
+clear X5 H1.
+inversion X3;subst.
+inversion X5;subst.
+inversion H12;subst.
+destruct vs; inversion H1.
 inversion X7;subst.
 inversion X8;subst.
-inversion H1;subst.
-clear H1 X8.
-inversion X1;subst.
-inversion X8;subst.
-inversion H12;subst.
-destruct vs; inversion H1.
-inversion H12;subst.
-destruct vs; inversion H1.
+inversion X9;subst.
 inversion X10;subst.
-inversion X11;subst.
+inversion H1;subst.
+clear X10 H1.
+inversion X6;subst.
+inversion X10;subst.
+inversion H12;subst.
+destruct vs; inversion H1.
 inversion X12;subst.
 inversion X13;subst.
-clear H1 X13.
-inversion X9;subst.
-inversion X13;subst.
+inversion X11;subst.
+inversion X14;subst.
 inversion H12;subst.
-destruct vs; inversion H1.
-inversion H12;subst.
-destruct vs; inversion H1.
+destruct vs; inversion H1;subst.
+destruct vs; inversion H4;subst.
+clear H4 H1 H13.
+unfold mkVEnv in *.
+simpl in *.
 inversion X15;subst.
 inversion X16;subst.
-admit.
-inversion X17.
-inversion X15.
-inversion X10.
-inversion X5.
-*)
-clear X IHn k3 k2 k1 t tenv ftenv idx.
+inversion X18;subst.
+inversion X19;subst.
+inversion X20;subst.
+inversion X21;subst.
+inversion H1;subst.
+repeat apply inj_pair2 in H7.
+subst.
+inversion X15;subst.
+inversion X22;subst.
+
+
+clear X15 X14 X12 X11 X10 X9 X8 X7 X6 X5 X4 X3 X2 X1 X X0 H H1 H2 H3 H4 k4 k3 k2 k1 k0.
+intuition.
+case_eq (lt_dec i tableSize);intros; try contradiction.
+rewrite H3 in *.
+subst.
+
+clear X0 X1 X H k4 k3 k2 k1 k0 t ft ftenv ftenv0 tenv env idx.
 intros idx Hidx.
 intuition; simpl in *.
  assert (Hor : idx = {| i := i; Hi := Hi |} \/ idx < {| i := i; Hi := Hi |}).
@@ -457,14 +513,16 @@ instantiate (1:=s).
 destruct Hor.
 subst.
 assumption.
-apply H1;trivial.
+apply H;trivial..*)
 (** false case*)
+revert H.
+clear;intros.
 unfold mkVEnv in *.
 simpl in *.
 unfold THoareTriple_Eval.
 intros.
 intuition.
-clear IHn k3 k2 k1 t tenv ftenv.
+clear k3 k2 k1 ftenv tenv.
 inversion X;subst.
 Focus 2. inversion X0.
 inversion H4.
